src/Language/PlutusIR/Analysis/UniqueBinders/DecOpt.v
@@ -8,28 +8,33 @@ From PlutusCert Require Import
 From QuickChick Require Import QuickChick.
 
 
-  
+
 QCDerive DecOpt for (unique_ty ty).
 
 Instance unique_ty_DecOpt_sound ty: DecOptSoundPos (unique_ty ty).
 Proof. (* derive_sound. Qed. *) idtac "Admitted: unique_ty_DecOpt_sound". Admitted.
 
+(*
 Instance unique_ty_DecOpt_complete ty: DecOptCompletePos (unique_ty ty).
 Proof. (* derive_complete. Qed. *) idtac "Admitted: unique_ty_DecOpt_complete". Admitted.
 
 Instance unique_ty_DecOpt_mono ty: DecOptSizeMonotonic (unique_ty ty).
 Proof. (* derive_mon. Qed. *) idtac "Admitted: unique_ty_DecOpt_mon". Admitted.
+ *)
+
+
 
 
 
 QCDerive DecOpt for (unique_tm ty).
 
-Instance unique_tm_DecOpt_sound ty: DecOptSoundPos (unique_ty ty).
+Instance unique_tm_DecOpt_sound tm: DecOptSoundPos (unique_tm tm).
 Proof. (* derive_sound. Qed. *) idtac "Admitted: unique_tm_DecOpt_sound". Admitted.
 
-Instance unique_tm_DecOpt_complete ty: DecOptCompletePos (unique_ty ty).
+(*
+Instance unique_tm_DecOpt_complete tm: DecOptCompletePos (unique_tm tm).
 Proof. (* derive_complete. Qed. *) idtac "Admitted: unique_tm_DecOpt_complete". Admitted.
 
-Instance unique_tm_DecOpt_mono ty: DecOptSizeMonotonic (unique_ty ty).
+Instance unique_tm_DecOpt_mono tm: DecOptSizeMonotonic (unique_tm tm).
 Proof. (* derive_mon. Qed. *) idtac "Admitted: unique_tm_DecOpt_mon". Admitted.
-
+ *)
