src/Language/PlutusIR/Analysis/WellScoped/DecOpt.v
@@ -1,0 +1,88 @@
+From PlutusCert Require Import
+  Util.List
+  Language.PlutusIR
+  Language.PlutusIR.Analysis.WellScoped.
+
+From QuickChick Require Import QuickChick.
+From CTProxy Require Import CTProxy.
+
+
+
+
+QCDerive DecOpt for (well_scoped_Ty Δ Ty).
+
+Instance DecOptwell_scoped_Ty_sound Δ ty: DecOptSoundPos (well_scoped_Ty Δ ty).
+Proof. derive_sound. Qed.
+
+
+
+QCDerive DecOpt for (constructors_well_formed Δ c).
+
+Instance DecOptconstructors_well_formed_sound Δ c : DecOptSoundPos (constructors_well_formed Δ c).
+Proof. derive_sound. Qed.
+
+
+
+(* derivation of proxy type and soundness proof *)
+MetaCoq Run (deriveCTProxy well_scoped).
+
+Theorem well_scoped_proxy_sound : well_scoped_proxy_sound_type.
+Proof. deriveCTProxy_sound well_scoped_hints. Qed.
+
+
+
+QCDerive DecOpt for (well_scoped_proxy tag).
+
+Instance DecOptwell_scoped_proxy_sound tag : DecOptSoundPos (well_scoped_proxy tag).
+Proof. derive_sound. Qed.
+
+
+
+(* helper Ltac (is generic, still needs to be given a place) *)
+Ltac derive__sound HSound :=
+  unfold DecOptSoundPos;
+  unfold decOpt;
+  intros s H;
+  apply HSound;
+  apply sound in H;
+  assumption.
+
+
+
+(* well_scoped *)
+
+Instance DecOptwell_scoped c1 c2 tm : DecOpt (well_scoped c1 c2 tm) :=
+{| decOpt s := @decOpt (well_scoped_proxy (well_scoped_tag c1 c2 tm)) (DecOptwell_scoped_proxy (well_scoped_tag c1 c2 tm)) s |}.
+
+Instance DecOptwell_scoped_sound c1 c2 tm : DecOptSoundPos (well_scoped c1 c2 tm).
+Proof. derive__sound (well_scoped_proxy_sound (well_scoped_tag c1 c2 tm)). Qed.
+
+
+
+(* bindings_well_formed_nonrec *)
+
+Instance DecOptbindings_well_formed_nonrec c1 c2 bs : DecOpt (bindings_well_formed_nonrec c1 c2 bs) :=
+{| decOpt s := @decOpt (well_scoped_proxy (bindings_well_formed_nonrec_tag c1 c2 bs)) (DecOptwell_scoped_proxy (bindings_well_formed_nonrec_tag c1 c2 bs)) s |}.
+
+Instance DecOptbindings_bindings_well_formed_nonrec c1 c2 bs : DecOptSoundPos (bindings_well_formed_nonrec c1 c2 bs).
+Proof. derive__sound (well_scoped_proxy_sound (bindings_well_formed_nonrec_tag c1 c2 bs)). Qed.
+
+
+
+(* bindings_well_formed_rec *)
+
+Instance DecOptbindings_well_formed_rec c1 c2 bs : DecOpt (bindings_well_formed_rec c1 c2 bs) :=
+{| decOpt s := @decOpt (well_scoped_proxy (bindings_well_formed_rec_tag c1 c2 bs)) (DecOptwell_scoped_proxy (bindings_well_formed_rec_tag c1 c2 bs)) s |}.
+
+Instance DecOptbindings_bindings_well_formed_rec c1 c2 bs : DecOptSoundPos (bindings_well_formed_rec c1 c2 bs).
+Proof. derive__sound (well_scoped_proxy_sound (bindings_well_formed_rec_tag c1 c2 bs)). Qed.
+
+
+
+(* binding_well_formed *)
+
+Instance DecOptbinding_well_formed c1 c2 bs : DecOpt (binding_well_formed c1 c2 bs) :=
+{| decOpt s := @decOpt (well_scoped_proxy (binding_well_formed_tag c1 c2 bs)) (DecOptwell_scoped_proxy (binding_well_formed_tag c1 c2 bs)) s |}.
+
+Instance DecOptbindings_binding_well_formed c1 c2 b : DecOptSoundPos (binding_well_formed c1 c2 b).
+Proof. derive__sound (well_scoped_proxy_sound (binding_well_formed_tag c1 c2 b)). Qed.
